src/ssa/opsem_inst.v
@@ -26,250 +26,8 @@ Require Import Floats.
 Require Import AST.
 Require Import Maps.
 Require Import opsem.
-
-Module OpsemProps (GVsSig : GenericValuesSig).
-
-Module OS := Opsem GVsSig.
-Export OS.
-
-Lemma BOP_inversion : forall TD lc gl b s v1 v2 gv2,
-  BOP TD lc gl b s v1 v2 = Some gv2 ->
-  exists gvs1, exists gvs2,
-    getOperandValue TD v1 lc gl = Some gvs1 /\
-    getOperandValue TD v2 lc gl = Some gvs2 /\
-    GVsSig.lift_op2 (mbop TD b s) gvs1 gvs2 (typ_int s) = gv2.
-Proof.
-  intros TD lc gl b s v1 v2 gv2 HBOP.
-  unfold BOP in HBOP.
-  remember (getOperandValue TD v1 lc gl) as ogv1.
-  destruct ogv1; try solve [inversion HBOP]. 
-  remember (getOperandValue TD v2 lc gl) as ogv2.
-  destruct ogv2; inv HBOP.
-  eauto.
-Qed.
-
-Lemma FBOP_inversion : forall TD lc gl b fp v1 v2 gv,
-  FBOP TD lc gl b fp v1 v2 = Some gv ->
-  exists gv1, exists gv2,
-    getOperandValue TD v1 lc gl = Some gv1 /\
-    getOperandValue TD v2 lc gl = Some gv2 /\
-    GVsSig.lift_op2 (mfbop TD b fp) gv1 gv2 (typ_floatpoint fp) = gv.
-Proof.
-  intros TD lc gl b fp v1 v2 gv HFBOP.
-  unfold FBOP in HFBOP.
-  remember (getOperandValue TD v1 lc gl) as ogv1.
-  destruct ogv1; try solve [inversion HFBOP].
-  remember (getOperandValue TD v2 lc gl) as ogv2.
-  destruct ogv2; inv HFBOP.
-  eauto.
-Qed.
-
-Lemma CAST_inversion : forall TD lc gl op t1 v1 t2 gv,
-  CAST TD lc gl op t1 v1 t2 = Some gv ->
-  exists gv1,
-    getOperandValue TD v1 lc gl = Some gv1 /\
-    GVsSig.lift_op1 (mcast TD op t1 t2) gv1 t2 = gv.
-Proof.
-  intros TD lc gl op t1 v1 t2 gv HCAST.
-  unfold CAST in HCAST.
-  remember (getOperandValue TD v1 lc gl) as ogv1.
-  destruct ogv1; inv HCAST.
-  eauto.
-Qed.
-
-Lemma TRUNC_inversion : forall TD lc gl op t1 v1 t2 gv,
-  TRUNC TD lc gl op t1 v1 t2 = Some gv ->
-  exists gv1,
-    getOperandValue TD v1 lc gl = Some gv1 /\
-    GVsSig.lift_op1 (mtrunc TD op t1 t2) gv1 t2 = gv.
-Proof.
-  intros TD lc gl op t1 v1 t2 gv HTRUNC.
-  unfold TRUNC in HTRUNC.
-  remember (getOperandValue TD v1 lc gl) as ogv1.
-  destruct ogv1; inv HTRUNC.
-  eauto.
-Qed.
-
-Lemma EXT_inversion : forall TD lc gl op t1 v1 t2 gv,
-  EXT TD lc gl op t1 v1 t2 = Some gv ->
-  exists gv1,
-    getOperandValue TD v1 lc gl = Some gv1 /\
-    GVsSig.lift_op1 (mext TD op t1 t2) gv1 t2 = gv.
-Proof.
-  intros TD lc gl op t1 v1 t2 gv HEXT.
-  unfold EXT in HEXT.
-  remember (getOperandValue TD v1 lc gl) as ogv1.
-  destruct ogv1; inv HEXT.
-  eauto.
-Qed.
-
-Lemma ICMP_inversion : forall TD lc gl cond t v1 v2 gv,
-  ICMP TD lc gl cond t v1 v2 = Some gv ->
-  exists gv1, exists gv2,
-    getOperandValue TD v1 lc gl = Some gv1 /\
-    getOperandValue TD v2 lc gl = Some gv2 /\
-    GVsSig.lift_op2 (micmp TD cond t) gv1 gv2 (typ_int 1%nat) = gv.
-Proof.
-  intros TD lc gl cond0 t v1 v2 gv HICMP.
-  unfold ICMP in HICMP.
-  remember (getOperandValue TD v1 lc gl) as ogv1.
-  destruct ogv1; try solve [inversion HICMP].
-  remember (getOperandValue TD v2 lc gl) as ogv2.
-  destruct ogv2; inv HICMP.
-  eauto.
-Qed.
-
-Lemma FCMP_inversion : forall TD lc gl cond fp v1 v2 gv,
-  FCMP TD lc gl cond fp v1 v2 = Some gv ->
-  exists gv1, exists gv2,
-    getOperandValue TD v1 lc gl = Some gv1 /\
-    getOperandValue TD v2 lc gl = Some gv2 /\
-    GVsSig.lift_op2 (mfcmp TD cond fp) gv1 gv2 (typ_int 1%nat) = gv.
-Proof.
-  intros TD lc gl cond0 fp v1 v2 gv HFCMP.
-  unfold FCMP in HFCMP.
-  remember (getOperandValue TD v1 lc gl) as ogv1.
-  destruct ogv1; try solve [inversion HFCMP].
-  remember (getOperandValue TD v2 lc gl) as ogv2.
-  destruct ogv2; inv HFCMP.
-  eauto.
-Qed.
-
-(*
-Lemma GEP_inversion : forall (TD:TargetData) (t:typ) (ma:GenericValue) 
-  (vidxs:list GenericValue) ib mptr0,
-  GEP TD t ma vidxs ib = Some mptr0 ->
-  exists idxs, exists ptr, exists ptr0, 
-    GVs2Nats TD vidxs = Some idxs /\ 
-    GV2ptr TD (getPointerSize TD) ma = Some ptr /\
-    mgep TD t ptr idxs = Some ptr0 /\
-    ptr2GV TD ptr0 = mptr0.
-Proof.
-  intros.
-  unfold GEP in H.
-  remember (GVs2Nats TD vidxs) as oidxs.
-  remember (GV2ptr TD (getPointerSize TD) ma) as R.
-  destruct R.
-    destruct oidxs.
-      remember (mgep TD t v l0) as og.
-      destruct og; inversion H; subst.
-        exists l0. exists v. exists v0. auto.
-        exists l0. exists v. exists v0. auto.
-
-Qed.
-*)
-
-Lemma const2GV_eqAL : forall c gl1 gl2 TD, 
-  eqAL _ gl1 gl2 -> 
-  const2GV TD gl1 c = const2GV TD gl2 c.
-Proof.
-  intros. unfold const2GV.
-  destruct const2GV_eqAL_aux.
-  erewrite H0; eauto.
-Qed.
-
-Lemma getOperandValue_eqAL : forall lc1 gl lc2 v TD,
-  eqAL _ lc1 lc2 ->
-  getOperandValue TD v lc1 gl = getOperandValue TD v lc2 gl.
-Proof.
-  intros lc1 gl lc2 v TD HeqAL.
-  unfold getOperandValue in *.
-  destruct v; auto.
-Qed.
-
-Lemma BOP_eqAL : forall lc1 gl lc2 bop0 sz0 v1 v2 TD,
-  eqAL _ lc1 lc2 ->
-  BOP TD lc1 gl bop0 sz0 v1 v2 = BOP TD lc2 gl bop0 sz0 v1 v2.
-Proof.
-  intros lc1 gl lc2 bop0 sz0 v1 v2 TD HeqEnv.
-  unfold BOP in *.
-  rewrite getOperandValue_eqAL with (lc2:=lc2)(v:=v1); auto.
-  rewrite getOperandValue_eqAL with (lc2:=lc2)(v:=v2); auto.
-Qed.
-
-Lemma FBOP_eqAL : forall lc1 gl lc2 fbop0 fp0 v1 v2 TD,
-  eqAL _ lc1 lc2 ->
-  FBOP TD lc1 gl fbop0 fp0 v1 v2 = FBOP TD lc2 gl fbop0 fp0 v1 v2.
-Proof.
-  intros lc1 gl lc2 fbop0 fp0 v1 v2 TD HeqEnv.
-  unfold FBOP in *.
-  rewrite getOperandValue_eqAL with (lc2:=lc2)(v:=v1); auto.
-  rewrite getOperandValue_eqAL with (lc2:=lc2)(v:=v2); auto.
-Qed.
-
-Lemma CAST_eqAL : forall lc1 gl lc2 op t1 v1 t2 TD,
-  eqAL _ lc1 lc2 ->
-  CAST TD lc1 gl op t1 v1 t2 = CAST TD lc2 gl op t1 v1 t2.
-Proof.
-  intros lc1 gl lc2 op t1 v1 t2 TD HeqAL.
-  unfold CAST in *.
-  rewrite getOperandValue_eqAL with (lc2:=lc2)(v:=v1); auto.
-Qed.
-
-Lemma TRUNC_eqAL : forall lc1 gl lc2 op t1 v1 t2 TD,
-  eqAL _ lc1 lc2 ->
-  TRUNC TD lc1 gl op t1 v1 t2 = TRUNC TD lc2 gl op t1 v1 t2.
-Proof.
-  intros lc1 gl lc2 op t1 v1 t2 TD HeqAL.
-  unfold TRUNC in *.
-  rewrite getOperandValue_eqAL with (lc2:=lc2)(v:=v1); auto.
-Qed.
-
-Lemma EXT_eqAL : forall lc1 gl lc2 op t1 v1 t2 TD,
-  eqAL _ lc1 lc2 ->
-  EXT TD lc1 gl op t1 v1 t2 = EXT TD lc2 gl op t1 v1 t2.
-Proof.
-  intros lc1 gl lc2 op t1 v1 t2 TD HeqAL.
-  unfold EXT in *.
-  rewrite getOperandValue_eqAL with (lc2:=lc2)(v:=v1); auto.
-Qed.
-
-Lemma ICMP_eqAL : forall lc1 gl lc2 cond t v1 v2 TD,
-  eqAL _ lc1 lc2 ->
-  ICMP TD lc1 gl cond t v1 v2 = ICMP TD lc2 gl cond t v1 v2.
-Proof.
-  intros lc1 gl lc2 cond0 t v1 v2 TD HeqAL.
-  unfold ICMP in *.
-  rewrite getOperandValue_eqAL with (lc2:=lc2)(v:=v1); auto.
-  rewrite getOperandValue_eqAL with (lc2:=lc2)(v:=v2); auto.
-Qed.
-
-Lemma FCMP_eqAL : forall lc1 gl lc2 cond fp v1 v2 TD,
-  eqAL _ lc1 lc2 ->
-  FCMP TD lc1 gl cond fp v1 v2 = FCMP TD lc2 gl cond fp v1 v2.
-Proof.
-  intros lc1 gl lc2 cond0 fp v1 v2 TD HeqAL.
-  unfold FCMP in *.
-  rewrite getOperandValue_eqAL with (lc2:=lc2)(v:=v1); auto.
-  rewrite getOperandValue_eqAL with (lc2:=lc2)(v:=v2); auto.
-Qed.
-
-Lemma values2GVs_eqAL : forall l0 lc1 gl lc2 TD,
-  eqAL _ lc1 lc2 ->
-  values2GVs TD l0 lc1 gl = values2GVs TD l0 lc2 gl.
-Proof.
-  induction l0; intros lc1 gl lc2 TD HeqAL; simpl; auto.
-    rewrite getOperandValue_eqAL with (lc2:=lc2)(v:=v); auto.
-    erewrite IHl0; eauto.
-Qed.
-(*
-Lemma lookupFdefViaGV_inversion : forall TD Ps gl lc fs fv f,
-  lookupFdefViaGV TD Ps gl lc fs fv = Some f ->
-  exists fptr, exists fn,
-    getOperandValue TD fv lc gl = Some fptr /\
-    lookupFdefViaGVFromFunTable fs fptr = Some fn /\
-    lookupFdefViaIDFromProducts Ps fn = Some f.
-Proof.
-  intros.
-  unfold lookupFdefViaGV in H.
-  destruct (getOperandValue TD fv lc gl); tinv H.
-  simpl in H. exists g.
-  destruct (lookupFdefViaGVFromFunTable fs g); tinv H.
-  simpl in H. exists i0. eauto.
-Qed.  
-*)
-
-End OpsemProps.
+Require Import opsem_props.
+Require Import dopsem.
 
 (************** Instantiate GVs ******************)
 
@@ -471,22 +229,23 @@ Proof.
     destruct gv; auto using singleton_inhabited, undef_gvs__inhabited.
 Qed.
 
-Definition lift_op1 (f: GenericValue -> option GenericValue) gvs1 ty : t :=
-  fun gv2 => exists gv1, exists gv2', 
-    gv1 @ gvs1 /\ f gv1 = Some gv2' /\ (gv2 @ $ gv2' # ty $).
+Definition lift_op1 (f: GenericValue -> option GenericValue) gvs1 ty : option t 
+  :=
+  Some (fun gv2 => exists gv1, exists gv2', 
+    gv1 @ gvs1 /\ f gv1 = Some gv2' /\ (gv2 @ $ gv2' # ty $)).
 
 Definition lift_op2 (f: GenericValue -> GenericValue -> option GenericValue)
-  gvs1 gvs2 ty : t :=
-  fun gv3 => exists gv1, exists gv2, exists gv3',
-    gv1 @ gvs1 /\ gv2 @ gvs2 /\ f gv1 gv2 = Some gv3' /\ (gv3 @ $ gv3' # ty $).
+  gvs1 gvs2 ty : option t :=
+  Some (fun gv3 => exists gv1, exists gv2, exists gv3',
+    gv1 @ gvs1 /\ gv2 @ gvs2 /\ f gv1 gv2 = Some gv3' /\ (gv3 @ $ gv3' # ty $)).
 
-Lemma lift_op1__inhabited : forall f gvs1 ty
+Lemma lift_op1__inhabited : forall f gvs1 ty gvs2
   (H:forall x, exists z, f x = Some z),
-  inhabited gvs1 -> inhabited (lift_op1 f gvs1 ty).
+  inhabited gvs1 -> 
+  lift_op1 f gvs1 ty = Some gvs2 -> 
+  inhabited gvs2.
 Proof.
-  intros.
-  unfold lift_op1. 
-  inv H0.
+  intros. inv H1. inv H0.
   destruct (@H x) as [z J].
   destruct (@gv2gvs__inhabited z ty).
   exists x0. unfold Ensembles.In. exists x. exists z.
@@ -494,14 +253,13 @@ Proof.
   repeat (split; auto).
 Qed.
 
-Lemma lift_op2__inhabited : forall f gvs1 gvs2 ty
+Lemma lift_op2__inhabited : forall f gvs1 gvs2 ty gv3
   (H:forall x y, exists z, f x y = Some z),
-  inhabited gvs1 -> Ensembles.Inhabited _ gvs2 ->
-  inhabited (lift_op2 f gvs1 gvs2 ty).
+  inhabited gvs1 -> inhabited gvs2 ->
+  lift_op2 f gvs1 gvs2 ty = Some gv3 ->
+  inhabited gv3.
 Proof.
-  intros.
-  unfold lift_op2. 
-  inv H0. inv H1.
+  intros. inv H0. inv H1. inv H2.
   destruct (@H x x0) as [z J].
   destruct (@gv2gvs__inhabited z ty).
   exists x1. unfold Ensembles.In. exists x. exists x0. exists z.
@@ -509,38 +267,52 @@ Proof.
   repeat (split; auto).
 Qed.
 
-Lemma lift_op1__getTypeSizeInBits : forall S los nts f g t sz al,
+Lemma lift_op1__isnt_stuck : forall f gvs1 ty
+  (H:forall x, exists z, f x = Some z),
+  exists gvs2, lift_op1 f gvs1 ty = Some gvs2.
+Proof.
+  intros. unfold lift_op1. eauto.
+Qed.
+
+Lemma lift_op2__isnt_stuck : forall f gvs1 gvs2 ty
+  (H:forall x y, exists z, f x y = Some z),
+  exists gv3, lift_op2 f gvs1 gvs2 ty = Some gv3.
+Proof.
+  intros. unfold lift_op2. eauto.
+Qed.
+
+Lemma lift_op1__getTypeSizeInBits : forall S los nts f g t sz al gvs,
   wf_typ S t ->
   _getTypeSizeInBits_and_Alignment los 
     (getTypeSizeInBits_and_Alignment_for_namedts (los,nts) true) true t = 
       Some (sz, al) ->
   (forall x y, x @ g -> f x = Some y -> 
    sizeGenericValue y = nat_of_Z (ZRdiv (Z_of_nat sz) 8)) ->
+  lift_op1 f g t = Some gvs ->
   forall gv : GenericValue,
-  gv @ lift_op1 f g t ->
+  gv @ gvs ->
   sizeGenericValue gv = nat_of_Z (ZRdiv (Z_of_nat sz) 8).
 Proof.
-  intros.
-  unfold lift_op1 in H2.
-  destruct H2 as [x [y [J1 [J2 J3]]]].
+  intros. inv H2.
+  destruct H3 as [x [y [J1 [J2 J3]]]].
   apply H1 in J2; auto.
   eapply gv2gvs__getTypeSizeInBits; eauto.
 Qed.
 
-Lemma lift_op2__getTypeSizeInBits : forall S los nts f g1 g2 t sz al,
+Lemma lift_op2__getTypeSizeInBits : forall S los nts f g1 g2 t sz al gvs,
   wf_typ S t ->
   _getTypeSizeInBits_and_Alignment los 
     (getTypeSizeInBits_and_Alignment_for_namedts (los,nts) true) true t = 
       Some (sz, al) ->
   (forall x y z, x @ g1 -> y @ g2 -> f x y = Some z -> 
    sizeGenericValue z = nat_of_Z (ZRdiv (Z_of_nat sz) 8)) ->
+  lift_op2 f g1 g2 t = Some gvs ->
   forall gv : GenericValue,
-  gv @ lift_op2 f g1 g2 t ->
+  gv @ gvs ->
   sizeGenericValue gv = nat_of_Z (ZRdiv (Z_of_nat sz) 8).
 Proof.
-  intros.
-  unfold lift_op2 in H2.
-  destruct H2 as [x [y [z [J1 [J2 [J3 J4]]]]]].
+  intros. inv H2.
+  destruct H3 as [x [y [z [J1 [J2 [J3 J4]]]]]].
   apply H1 in J3; auto.
   eapply gv2gvs__getTypeSizeInBits; eauto.
 Qed.
@@ -580,197 +352,9 @@ Qed.
 
 End NDGVs.
 
-Module DGVs <: GenericValuesSig.
-
-Export LLVMsyntax.
-Export LLVMgv.
-
-Definition t := option GenericValue.
-Definition Map := list (id * t).
-Definition instantiate_gvs (gv : GenericValue) (gvs : t) : Prop := gvs = Some gv.
-Definition inhabited (gvs : t) : Prop := gvs <> None.
-Definition cundef_gvs (gv:GenericValue) (ty:typ) : t := 
-  Some (LLVMgv.cundef_gv gv ty).
-Definition undef_gvs gv (ty:typ) : t := Some gv.
-Definition cgv2gvs (gv:GenericValue) (ty:typ) : t := Some (LLVMgv.cgv2gv gv ty).
-Definition gv2gvs (gv:GenericValue) (ty:typ) : t := Some gv.
-
-Hint Unfold instantiate_gvs inhabited.
-
-Notation "gv @ gvs" :=  
-  (instantiate_gvs gv gvs) (at level 43, right associativity).
-Notation "$ gv # t $" := (gv2gvs gv t) (at level 41).
-
-Lemma cundef_gvs__getTypeSizeInBits : forall S los nts gv ty sz al gv',
-  wf_typ S ty ->
-  _getTypeSizeInBits_and_Alignment los 
-    (getTypeSizeInBits_and_Alignment_for_namedts (los,nts) true) true ty = 
-      Some (sz, al) ->
-  Coqlib.nat_of_Z (Coqlib.ZRdiv (Z_of_nat sz) 8) = sizeGenericValue gv ->
-  gv' @ (cundef_gvs gv ty) ->
-  Coqlib.nat_of_Z (Coqlib.ZRdiv (Z_of_nat sz) 8) = 
-    sizeGenericValue gv'.
-Proof.
-  unfold instantiate_gvs. 
-  intros. inv H2.
-  eapply LLVMgv.cundef_gv__getTypeSizeInBits; eauto.
-Qed.
-
-Lemma cundef_gvs__inhabited : forall gv ty, inhabited (cundef_gvs gv ty).
-Proof. intros. unfold cundef_gvs, inhabited. congruence. Qed.
-
-Lemma undef_gvs__getTypeSizeInBits : forall S los nts gv t sz al gv',
-  wf_typ S t ->
-  _getTypeSizeInBits_and_Alignment los 
-    (getTypeSizeInBits_and_Alignment_for_namedts (los,nts) true) true t = 
-      Some (sz, al) ->
-  Coqlib.nat_of_Z (Coqlib.ZRdiv (Z_of_nat sz) 8) = sizeGenericValue gv ->
-  gv' @ (undef_gvs gv t) ->
-  Coqlib.nat_of_Z (Coqlib.ZRdiv (Z_of_nat sz) 8) = 
-    sizeGenericValue gv'.
-Proof. 
-  unfold instantiate_gvs. 
-  intros. inv H2. auto.
-Qed.
-
-Lemma undef_gvs__inhabited : forall gv ty, inhabited (undef_gvs gv ty).
-Proof. intros. unfold undef_gvs, inhabited. congruence. Qed.
-
-Lemma cgv2gvs__getTypeSizeInBits : forall S los nts gv t sz al gv',
-  wf_typ S t ->
-  _getTypeSizeInBits_and_Alignment los 
-    (getTypeSizeInBits_and_Alignment_for_namedts (los,nts) true) true t = 
-      Some (sz, al) ->
-  Coqlib.nat_of_Z (Coqlib.ZRdiv (Z_of_nat sz) 8) = sizeGenericValue gv ->
-  gv' @ (cgv2gvs gv t) ->
-  Coqlib.nat_of_Z (Coqlib.ZRdiv (Z_of_nat sz) 8) = 
-    sizeGenericValue gv'.
-Proof.
-  unfold instantiate_gvs. 
-  intros. inv H2.
-  eapply LLVMgv.cgv2gv__getTypeSizeInBits; eauto.
-Qed.
-
-Lemma cgv2gvs__inhabited : forall gv t, inhabited (cgv2gvs gv t).
-Proof. intros. unfold cgv2gvs, inhabited. congruence. Qed.
-
-Lemma gv2gvs__getTypeSizeInBits : forall S los nts gv t sz al,
-  wf_typ S t ->
-  _getTypeSizeInBits_and_Alignment los 
-    (getTypeSizeInBits_and_Alignment_for_namedts (los,nts) true) true t = 
-      Some (sz, al) ->
-  Coqlib.nat_of_Z (Coqlib.ZRdiv (Z_of_nat sz) 8) = sizeGenericValue gv ->
-  forall gv', gv' @ (gv2gvs gv t) ->
-  sizeGenericValue gv' = Coqlib.nat_of_Z (Coqlib.ZRdiv (Z_of_nat sz) 8).
-Proof.
-  unfold instantiate_gvs. 
-  intros. inv H2. auto.
-Qed.
-
-Lemma gv2gvs__inhabited : forall gv t, inhabited ($ gv # t $).
-Proof. intros. unfold gv2gvs, inhabited. congruence. Qed.
-
-Definition lift_op1 (f: GenericValue -> option GenericValue) gvs1 (ty:typ) : t :=
-match gvs1 with
-| Some gv1 => f gv1
-| _ => None
-end.
-
-Definition lift_op2 (f: GenericValue -> GenericValue -> option GenericValue)
-  gvs1 gvs2 (ty: typ) : t := 
-match gvs1, gvs2 with
-| Some gv1, Some gv2 => f gv1 gv2
-| _, _ => None
-end.
-
-Lemma lift_op1__inhabited : forall f gvs1 ty
-  (H:forall x, exists z, f x = Some z),
-  inhabited gvs1 -> inhabited (lift_op1 f gvs1 ty).
-Proof.
-  intros.
-  unfold lift_op1. 
-  destruct gvs1; eauto.
-  destruct (@H g) as [z J].
-  rewrite J. congruence.
-Qed.
-
-Lemma lift_op2__inhabited : forall f gvs1 gvs2 t
-  (H:forall x y, exists z, f x y = Some z),
-  inhabited gvs1 -> inhabited gvs2 ->
-  inhabited (lift_op2 f gvs1 gvs2 t).
-Proof.
-  intros.
-  unfold lift_op2. 
-  destruct gvs1; eauto.
-  destruct gvs2; eauto.
-  destruct (@H g g0) as [z J].
-  rewrite J. congruence.
-Qed.
-
-Lemma lift_op1__getTypeSizeInBits : forall S los nts f g t sz al,
-  wf_typ S t ->
-  _getTypeSizeInBits_and_Alignment los 
-    (getTypeSizeInBits_and_Alignment_for_namedts (los,nts) true) true t = 
-      Some (sz, al) ->
-  (forall x y, x @ g -> f x = Some y -> 
-   sizeGenericValue y = nat_of_Z (ZRdiv (Z_of_nat sz) 8)) ->
-  forall gv : GenericValue,
-  gv @ lift_op1 f g t ->
-  sizeGenericValue gv = nat_of_Z (ZRdiv (Z_of_nat sz) 8).
-Proof.
-  intros.
-  unfold lift_op1, instantiate_gvs in H2.
-  destruct g; tinv H2.
-  apply H1 in H2; auto.
-Qed.
-
-Lemma lift_op2__getTypeSizeInBits : forall S los nts f g1 g2 t sz al,
-  wf_typ S t ->
-  _getTypeSizeInBits_and_Alignment los 
-    (getTypeSizeInBits_and_Alignment_for_namedts (los,nts) true) true t = 
-      Some (sz, al) ->
-  (forall x y z, x @ g1 -> y @ g2 -> f x y = Some z -> 
-   sizeGenericValue z = nat_of_Z (ZRdiv (Z_of_nat sz) 8)) ->
-  forall gv : GenericValue,
-  gv @ lift_op2 f g1 g2 t ->
-  sizeGenericValue gv = nat_of_Z (ZRdiv (Z_of_nat sz) 8).
-Proof.
-  intros.
-  unfold lift_op2, instantiate_gvs in H2.
-  destruct g1; tinv H2.
-  destruct g2; tinv H2.
-  apply H1 in H2; auto.
-Qed.
-
-Lemma inhabited_inv : forall gvs, inhabited gvs -> exists gv, gv @ gvs.
-Proof.
-  intros. 
-  destruct gvs; eauto.
-    congruence.
-Qed.
-
-Lemma instantiate_undef__undef_gvs : forall gv t, gv @ (undef_gvs gv t).
-Proof. auto. Qed.
-
-Lemma instantiate_gv__gv2gvs : forall gv t, gv @ ($ gv # t $).
-Proof. auto. Qed.
-
-Lemma none_undef2gvs_inv : forall gv gv' t,
-  gv @ $ gv' # t $ -> (forall mc, (Vundef, mc)::nil <> gv') -> gv = gv'.
-Proof.
-  intros.
-  destruct gv'; try solve [inv H; auto].
-Qed.
-
-End DGVs.
-
 Module NDOS := Opsem NDGVs.
 
-Module DOS := Opsem DGVs.
-
 Module OpsemInstantiation.
-
-Module DOSprop1 := OpsemProps DGVs.
 
 Definition instantiate_gvs (gvs1:DGVs.t) (gvs2: NDGVs.t) : Prop :=
 forall gv1, 
@@ -821,29 +405,50 @@ Proof.
                exists Float.zero; auto]].
 Qed.
 
-Lemma instantiate_gvs__lift_op1 : forall f xs1 xs2 t,
+Lemma instantiate_gvs__lift_op1 : forall f xs1 xs2 t ys1,
   instantiate_gvs xs1 xs2 ->
-  instantiate_gvs (DGVs.lift_op1 f xs1 t) (NDGVs.lift_op1 f xs2 t).
+  DGVs.lift_op1 f xs1 t = Some ys1 ->
+  exists ys2, NDGVs.lift_op1 f xs2 t = Some ys2 /\ instantiate_gvs ys1 ys2.
 Proof.
-  intros.
   unfold DGVs.lift_op1, NDGVs.lift_op1.
-  destruct xs1; intros gvs1 J; inv J.
-    exists g. exists gvs1. 
-    repeat (split; auto using NDGVs.instantiate_gv__gv2gvs).
+  intros.
+  exists (fun gv2 : GenericValue =>
+          exists gv1 : GenericValue,
+            exists gv2' : GenericValue,
+              NDGVs.instantiate_gvs gv1 xs2 /\
+              f gv1 = ret gv2' /\
+              NDGVs.instantiate_gvs gv2 (NDGVs.gv2gvs gv2' t)).
+  split; auto.
+  exists xs1. exists gv1. inv H1.
+  repeat (split; eauto using NDGVs.instantiate_gv__gv2gvs).
 Qed.
 
-Lemma instantiate_gvs__lift_op2 : forall f xs1 ys1 xs2 ys2 t,
+Lemma instantiate_gvs__lift_op2 : forall f xs1 ys1 xs2 ys2 t zxs1,
   instantiate_gvs xs1 xs2 ->
   instantiate_gvs ys1 ys2 ->
-  instantiate_gvs (DGVs.lift_op2 f xs1 ys1 t) (NDGVs.lift_op2 f xs2 ys2 t).
+  DGVs.lift_op2 f xs1 ys1 t = Some zxs1 ->
+  exists zxs2, NDGVs.lift_op2 f xs2 ys2 t = Some zxs2 /\ 
+    instantiate_gvs zxs1 zxs2.
 Proof.
-  intros.
   unfold DGVs.lift_op2, NDGVs.lift_op2.
-  destruct xs1; intros gvs1 J; inv J.
-  destruct ys1; tinv H2.
-    exists g. exists g0. exists gvs1. 
-    repeat (split; auto using NDGVs.instantiate_gv__gv2gvs).
+  intros.
+  exists (fun gv3 : GenericValue =>
+          exists gv1 : GenericValue,
+            exists gv2 : GenericValue,
+              exists gv3' : GenericValue,
+                NDGVs.instantiate_gvs gv1 xs2 /\
+                NDGVs.instantiate_gvs gv2 ys2 /\
+                f gv1 gv2 = ret gv3' /\
+                NDGVs.instantiate_gvs gv3 (NDGVs.gv2gvs gv3' t)).
+  split; auto.
+  exists xs1. exists ys1. exists zxs1. inv H2.
+  repeat (split; eauto using NDGVs.instantiate_gv__gv2gvs).
 Qed.
+
+Global Opaque NDGVs.instantiate_gvs NDGVs.inhabited NDGVs.cgv2gvs NDGVs.gv2gvs
+  NDGVs.lift_op1 NDGVs.lift_op2 NDGVs.t
+  DGVs.instantiate_gvs DGVs.inhabited DGVs.cgv2gvs DGVs.gv2gvs
+  DGVs.lift_op1 DGVs.lift_op2 DGVs.t.
 
 Fixpoint instantiate_locals (lc1 : DOS.GVsMap) (lc2 : NDOS.GVsMap) : Prop :=
 match lc1, lc2 with
@@ -948,11 +553,13 @@ Proof.
   rewrite J1. 
   destruct c; tinv H1.
   destruct n; inv H1; eauto.
-  destruct t; inv H3.
-  exists (updateAddAL _ lc2' i0 (NDGVs.lift_op1 (fit_gv TD t) gvs2 t)).   
-  split; auto.
-    apply instantiate_locals__updateAddAL; auto.
-    apply instantiate_gvs__lift_op1; auto.
+  destruct t; tinv H3.
+  remember (DGVs.lift_op1 (fit_gv TD t) g t) as R.
+  destruct R as [gr'|]; inv H3.
+  symmetry in HeqR.
+  eapply instantiate_gvs__lift_op1 in HeqR; eauto.
+  destruct HeqR as [ys2 [J3 J4]]. rewrite J3.
+  eauto using instantiate_locals__updateAddAL.
 Qed.
 
 Lemma instantiate_locals__getIncomingValuesForBlockFromPHINodes : forall TD b
@@ -1020,7 +627,7 @@ Lemma instantiate_locals__BOP : forall TD lc1 lc2 gl v1 v2 gvs3 bop sz,
     instantiate_gvs gvs3 gvs3'.
 Proof.
   intros.
-  apply DOSprop1.BOP_inversion in H0.
+  apply DOSprop.BOP_inversion in H0.
   destruct H0 as [gv1 [gv2 [J1 [J2 J3]]]]; subst.
   eapply instantiate_locals__getOperandValue in J1; eauto.
   destruct J1 as [gvs1 [H1 H2]].
@@ -1038,7 +645,7 @@ Lemma instantiate_locals__FBOP : forall TD lc1 lc2 gl v1 v2 gv3 fbop fp,
     instantiate_gvs gv3 gvs3'.
 Proof.
   intros.
-  apply DOSprop1.FBOP_inversion in H0.
+  apply DOSprop.FBOP_inversion in H0.
   destruct H0 as [gv1 [gv2 [J1 [J2 J3]]]]; subst.
   eapply instantiate_locals__getOperandValue in J1; eauto.
   destruct J1 as [gvs1 [H1 H2]].
@@ -1056,7 +663,7 @@ Lemma instantiate_locals__ICMP : forall TD lc1 lc2 gl v1 v2 gv3 c t,
     instantiate_gvs gv3 gvs3'.
 Proof.
   intros.
-  apply DOSprop1.ICMP_inversion in H0.
+  apply DOSprop.ICMP_inversion in H0.
   destruct H0 as [gv1 [gv2 [J1 [J2 J3]]]]; subst.
   eapply instantiate_locals__getOperandValue in J1; eauto.
   destruct J1 as [gvs1 [H1 H2]].
@@ -1074,7 +681,7 @@ Lemma instantiate_locals__FCMP : forall TD lc1 lc2 gl v1 v2 gv3 c t,
     instantiate_gvs gv3 gvs3'.
 Proof.
   intros.
-  apply DOSprop1.FCMP_inversion in H0.
+  apply DOSprop.FCMP_inversion in H0.
   destruct H0 as [gv1 [gv2 [J1 [J2 J3]]]]; subst.
   eapply instantiate_locals__getOperandValue in J1; eauto.
   destruct J1 as [gvs1 [H1 H2]].
@@ -1136,10 +743,11 @@ Proof.
     Hgep.
   inv Hgep.
   unfold NDOS.GEP.
+  unfold DOS.GEP in H0.
+  eapply instantiate_gvs__lift_op1 in H0; eauto.
+  destruct H0 as [ys2 [J1 J2]].
   exists vidxs1.  
-  exists (NDGVs.lift_op1 (NDOS.gep TD t vidxs1 inbounds) mps2
-           (typ_pointer (typ_int 1%nat))).
-  split; eauto using instantiate_gvs__lift_op1, in_instantiate_list_gvs.
+  eauto using in_instantiate_list_gvs.
 Qed.
 
 Lemma instantiate_locals__extractGenericValue : forall TD lc1 lc2 t gv2
@@ -1182,7 +790,7 @@ Lemma instantiate_locals__CAST : forall TD lc1 lc2 gl t1 v1 t2 gv2 castop0,
     /\ instantiate_gvs gv2 gvs2'.
 Proof.
   intros.
-  apply DOSprop1.CAST_inversion in H0.
+  apply DOSprop.CAST_inversion in H0.
   destruct H0 as [gv1 [J1 J2]]; subst.
   eapply instantiate_locals__getOperandValue in J1; eauto.
   destruct J1 as [gvs1 [H1 H2]].
@@ -1198,7 +806,7 @@ Lemma instantiate_locals__TRUNC : forall TD lc1 lc2 gl t1 v1 t2 gv2 top0,
     /\ instantiate_gvs gv2 gvs2'.
 Proof.
   intros.
-  apply DOSprop1.TRUNC_inversion in H0.
+  apply DOSprop.TRUNC_inversion in H0.
   destruct H0 as [gv1 [J1 J2]]; subst.
   eapply instantiate_locals__getOperandValue in J1; eauto.
   destruct J1 as [gvs1 [H1 H2]].
@@ -1214,7 +822,7 @@ Lemma instantiate_locals__EXT : forall TD lc1 lc2 gl t1 v1 t2 gv2 top0,
     /\ instantiate_gvs gv2 gvs2'.
 Proof.
   intros.
-  apply DOSprop1.EXT_inversion in H0.
+  apply DOSprop.EXT_inversion in H0.
   destruct H0 as [gv1 [J1 J2]]; subst.
   eapply instantiate_locals__getOperandValue in J1; eauto.
   destruct J1 as [gvs1 [H1 H2]].
@@ -1271,13 +879,19 @@ Proof.
       simpl in H1.
       destruct gvs2; inv H1.
       remember (DOS._initializeFrameValues TD la gvs1 lc1) as R1.
-      destruct R1; inv H.
+      destruct R1; tinv H.
+      remember (DGVs.lift_op1 (fit_gv TD t) t0 t) as R2.
+      destruct R2; inv H.
       symmetry in HeqR1.
       eapply IHla in HeqR1; eauto.
       destruct HeqR1 as [lc2' [J1 J2]].
       rewrite J1.
-      eauto using instantiate_locals__updateAddAL, instantiate_gvs__lift_op1.
-Qed.           
+      symmetry in HeqR2.
+      eapply instantiate_gvs__lift_op1 in HeqR2; eauto.
+      destruct HeqR2 as [ys2 [J3 J4]].
+      rewrite J3.
+      eauto using instantiate_locals__updateAddAL.
+Qed. 
 
 Lemma instantiate_locals__initLocals : forall TD gvs1 gvss2 
   (H : instantiate_list_gvs gvs1 gvss2) la lc1,
@@ -1323,17 +937,6 @@ Proof.
   destruct R; inv H2.
   eauto using instantiate_locals__updateAddAL, instantiate_gvs__gv2gvs.
 Qed.
-
-Tactic Notation "sInsn_cases" tactic(first) tactic(c) :=
-  first;
-  [ c "sReturn" | c "sReturnVoid" | c "sBranch" | c "sBranch_uncond" |
-    c "sBop" | c "sFBop" | c "sExtractValue" | c "sInsertValue" |
-    c "sMalloc" | c "sFree" |
-    c "sAlloca" | c "sLoad" | c "sStore" | c "sGEP" |
-    c "sTrunc" | c "sExt" | 
-    c "sCast" | 
-    c "sIcmp" | c "sFcmp" | c "sSelect" |  
-    c "sCall" | c "sExCall" ].
 
 Ltac simpl_nd_llvmds :=
   match goal with
@@ -1574,6 +1177,8 @@ Case "sExCall". simpl_nd_llvmds.
                                     instantiate_list_gvs__incl.
     repeat (split; auto).
 Qed.
+
+End OpsemInstantiation.
 
 
 (*****************************)
