src/ssa/dopsem.v
@@ -1,0 +1,207 @@
+Add LoadPath "./ott".
+Add LoadPath "./monads".
+Add LoadPath "./compcert".
+Add LoadPath "../../../theory/metatheory_8.3".
+Require Import Metatheory.
+Require Import alist.
+Require Import monad.
+Require Import genericvalues.
+Require Import Values.
+Require Import Memory.
+Require Import Integers.
+Require Import Coqlib.
+Require Import ssa_def.
+Require Import opsem.
+Require Import opsem_props.
+
+Module DGVs <: GenericValuesSig.
+
+Export LLVMsyntax.
+Export LLVMgv.
+
+Definition t := GenericValue.
+Definition Map := list (id * t).
+Definition instantiate_gvs (gv : GenericValue) (gvs : t) : Prop := gvs = gv.
+Definition inhabited (gvs : t) : Prop := True.
+Definition cundef_gvs := LLVMgv.cundef_gv.
+Definition undef_gvs gv (ty:typ) : t := gv.
+Definition cgv2gvs := LLVMgv.cgv2gv.
+Definition gv2gvs (gv:GenericValue) (ty:typ) : t := gv.
+
+Hint Unfold instantiate_gvs inhabited.
+
+Notation "gv @ gvs" :=  
+  (instantiate_gvs gv gvs) (at level 43, right associativity).
+Notation "$ gv # t $" := (gv2gvs gv t) (at level 41).
+
+Lemma cundef_gvs__getTypeSizeInBits : forall S los nts gv ty sz al gv',
+  wf_typ S ty ->
+  _getTypeSizeInBits_and_Alignment los 
+    (getTypeSizeInBits_and_Alignment_for_namedts (los,nts) true) true ty = 
+      Some (sz, al) ->
+  Coqlib.nat_of_Z (Coqlib.ZRdiv (Z_of_nat sz) 8) = sizeGenericValue gv ->
+  gv' @ (cundef_gvs gv ty) ->
+  Coqlib.nat_of_Z (Coqlib.ZRdiv (Z_of_nat sz) 8) = 
+    sizeGenericValue gv'.
+Proof.
+  unfold instantiate_gvs. 
+  intros. inv H2.
+  eapply LLVMgv.cundef_gv__getTypeSizeInBits; eauto.
+Qed.
+
+Lemma cundef_gvs__inhabited : forall gv ty, inhabited (cundef_gvs gv ty).
+Proof. auto. Qed.
+
+Lemma undef_gvs__getTypeSizeInBits : forall S los nts gv t sz al gv',
+  wf_typ S t ->
+  _getTypeSizeInBits_and_Alignment los 
+    (getTypeSizeInBits_and_Alignment_for_namedts (los,nts) true) true t = 
+      Some (sz, al) ->
+  Coqlib.nat_of_Z (Coqlib.ZRdiv (Z_of_nat sz) 8) = sizeGenericValue gv ->
+  gv' @ (undef_gvs gv t) ->
+  Coqlib.nat_of_Z (Coqlib.ZRdiv (Z_of_nat sz) 8) = 
+    sizeGenericValue gv'.
+Proof. 
+  unfold instantiate_gvs. 
+  intros. inv H2. auto.
+Qed.
+
+Lemma undef_gvs__inhabited : forall gv ty, inhabited (undef_gvs gv ty).
+Proof. auto. Qed.
+
+Lemma cgv2gvs__getTypeSizeInBits : forall S los nts gv t sz al gv',
+  wf_typ S t ->
+  _getTypeSizeInBits_and_Alignment los 
+    (getTypeSizeInBits_and_Alignment_for_namedts (los,nts) true) true t = 
+      Some (sz, al) ->
+  Coqlib.nat_of_Z (Coqlib.ZRdiv (Z_of_nat sz) 8) = sizeGenericValue gv ->
+  gv' @ (cgv2gvs gv t) ->
+  Coqlib.nat_of_Z (Coqlib.ZRdiv (Z_of_nat sz) 8) = 
+    sizeGenericValue gv'.
+Proof.
+  unfold instantiate_gvs. 
+  intros. inv H2.
+  eapply LLVMgv.cgv2gv__getTypeSizeInBits; eauto.
+Qed.
+
+Lemma cgv2gvs__inhabited : forall gv t, inhabited (cgv2gvs gv t).
+Proof. auto. Qed.
+
+Lemma gv2gvs__getTypeSizeInBits : forall S los nts gv t sz al,
+  wf_typ S t ->
+  _getTypeSizeInBits_and_Alignment los 
+    (getTypeSizeInBits_and_Alignment_for_namedts (los,nts) true) true t = 
+      Some (sz, al) ->
+  Coqlib.nat_of_Z (Coqlib.ZRdiv (Z_of_nat sz) 8) = sizeGenericValue gv ->
+  forall gv', gv' @ (gv2gvs gv t) ->
+  sizeGenericValue gv' = Coqlib.nat_of_Z (Coqlib.ZRdiv (Z_of_nat sz) 8).
+Proof.
+  unfold instantiate_gvs. 
+  intros. inv H2. auto.
+Qed.
+
+Lemma gv2gvs__inhabited : forall gv t, inhabited ($ gv # t $).
+Proof. auto. Qed.
+
+Definition lift_op1 (f: GenericValue -> option GenericValue) (gvs1:t) (ty:typ) : 
+  option t := f gvs1.
+
+Definition lift_op2 (f: GenericValue -> GenericValue -> option GenericValue)
+  (gvs1 gvs2:t) (ty: typ) : option t := f gvs1 gvs2.
+
+Lemma lift_op1__inhabited : forall f gvs1 ty gvs2
+  (H:forall x, exists z, f x = Some z),
+  inhabited gvs1 -> 
+  lift_op1 f gvs1 ty = Some gvs2 ->
+  inhabited gvs2.
+Proof. auto. Qed.
+
+Lemma lift_op2__inhabited : forall f gvs1 gvs2 t gvs3
+  (H:forall x y, exists z, f x y = Some z),
+  inhabited gvs1 -> inhabited gvs2 ->
+  lift_op2 f gvs1 gvs2 t = Some gvs3 ->
+  inhabited gvs3.
+Proof. auto. Qed.
+
+Lemma lift_op1__isnt_stuck : forall f gvs1 ty
+  (H:forall x, exists z, f x = Some z),
+  exists gvs2, lift_op1 f gvs1 ty = Some gvs2.
+Proof. unfold lift_op1. auto. Qed.
+
+Lemma lift_op2__isnt_stuck : forall f gvs1 gvs2 t
+  (H:forall x y, exists z, f x y = Some z),
+  exists gvs3, lift_op2 f gvs1 gvs2 t = Some gvs3.
+Proof. unfold lift_op2. auto. Qed.
+
+Lemma lift_op1__getTypeSizeInBits : forall S los nts f g t sz al gvs,
+  wf_typ S t ->
+  _getTypeSizeInBits_and_Alignment los 
+    (getTypeSizeInBits_and_Alignment_for_namedts (los,nts) true) true t = 
+      Some (sz, al) ->
+  (forall x y, x @ g -> f x = Some y -> 
+   sizeGenericValue y = nat_of_Z (ZRdiv (Z_of_nat sz) 8)) ->
+  lift_op1 f g t = Some gvs ->
+  forall gv : GenericValue,
+  gv @ gvs ->
+  sizeGenericValue gv = nat_of_Z (ZRdiv (Z_of_nat sz) 8).
+Proof. intros. unfold lift_op1 in H2. inv H3. eauto. Qed.
+
+Lemma lift_op2__getTypeSizeInBits : forall S los nts f g1 g2 t sz al gvs,
+  wf_typ S t ->
+  _getTypeSizeInBits_and_Alignment los 
+    (getTypeSizeInBits_and_Alignment_for_namedts (los,nts) true) true t = 
+      Some (sz, al) ->
+  (forall x y z, x @ g1 -> y @ g2 -> f x y = Some z -> 
+   sizeGenericValue z = nat_of_Z (ZRdiv (Z_of_nat sz) 8)) ->
+  lift_op2 f g1 g2 t = Some gvs ->
+  forall gv : GenericValue,
+  gv @ gvs ->
+  sizeGenericValue gv = nat_of_Z (ZRdiv (Z_of_nat sz) 8).
+Proof. intros. unfold lift_op2 in H2. inv H3. eauto. Qed.
+
+Lemma inhabited_inv : forall gvs, inhabited gvs -> exists gv, gv @ gvs.
+Proof. eauto. Qed.
+
+Lemma instantiate_undef__undef_gvs : forall gv t, gv @ (undef_gvs gv t).
+Proof. auto. Qed.
+
+Lemma instantiate_gv__gv2gvs : forall gv t, gv @ ($ gv # t $).
+Proof. auto. Qed.
+
+Lemma none_undef2gvs_inv : forall gv gv' t,
+  gv @ $ gv' # t $ -> (forall mc, (Vundef, mc)::nil <> gv') -> gv = gv'.
+Proof.
+  intros.
+  destruct gv'; try solve [inv H; auto].
+Qed.
+
+End DGVs.
+
+Module DOS := Opsem DGVs.
+
+Ltac dgvs_instantiate_inv :=
+  match goal with
+  | [ H : DGVs.instantiate_gvs _ _ |- _ ] => inv H
+  end.
+
+Lemma dos_in_list_gvs_intro : forall gvs, DOS.in_list_gvs gvs gvs.
+Proof. 
+  induction gvs; simpl; auto. 
+Qed.
+
+Lemma dos_in_list_gvs_inv : forall gvs gvss, 
+  DOS.in_list_gvs gvs gvss -> gvs = gvss.
+Proof.
+  induction 1; subst; try dgvs_instantiate_inv; auto. 
+Qed.
+
+Module DOSprop := OpsemProps DGVs.
+
+(*****************************)
+(*
+*** Local Variables: ***
+*** coq-prog-name: "coqtop" ***
+*** coq-prog-args: ("-emacs-U" "-I" "~/SVN/sol/vol/src/ssa/monads" "-I" "~/SVN/sol/vol/src/ssa/ott" "-I" "~/SVN/sol/vol/src/ssa/compcert" "-I" "~/SVN/sol/theory/metatheory_8.3") ***
+*** End: ***
+ *)
+
