src/ssa/opsem_props.v
@@ -1,0 +1,278 @@
+Add LoadPath "./ott".
+Add LoadPath "./monads".
+Add LoadPath "./compcert".
+Add LoadPath "../../../theory/metatheory_8.3".
+Require Import Ensembles.
+Require Import ssa_def.
+Require Import ssa_lib.
+Require Import ssa_props.
+Require Import ssa_analysis.
+Require Import ssa_static.
+Require Import ssa_static_lib.
+Require Import List.
+Require Import Arith.
+Require Import tactics.
+Require Import monad.
+Require Import trace.
+Require Import Metatheory.
+Require Import genericvalues.
+Require Import alist.
+Require Import Memory.
+Require Import Integers.
+Require Import Coqlib.
+Require Import targetdata.
+Require Import AST.
+Require Import Maps.
+Require Import opsem.
+
+Module OpsemProps (GVsSig : GenericValuesSig).
+
+Module OS := Opsem GVsSig.
+Export OS.
+
+Lemma BOP_inversion : forall TD lc gl b s v1 v2 gv2,
+  BOP TD lc gl b s v1 v2 = Some gv2 ->
+  exists gvs1, exists gvs2,
+    getOperandValue TD v1 lc gl = Some gvs1 /\
+    getOperandValue TD v2 lc gl = Some gvs2 /\
+    GVsSig.lift_op2 (mbop TD b s) gvs1 gvs2 (typ_int s) = Some gv2.
+Proof.
+  intros TD lc gl b s v1 v2 gv2 HBOP.
+  unfold BOP in HBOP.
+  remember (getOperandValue TD v1 lc gl) as ogv1.
+  destruct ogv1; try solve [inversion HBOP]. 
+  remember (getOperandValue TD v2 lc gl) as ogv2.
+  destruct ogv2; inv HBOP.
+  eauto.
+Qed.
+
+Lemma FBOP_inversion : forall TD lc gl b fp v1 v2 gv,
+  FBOP TD lc gl b fp v1 v2 = Some gv ->
+  exists gv1, exists gv2,
+    getOperandValue TD v1 lc gl = Some gv1 /\
+    getOperandValue TD v2 lc gl = Some gv2 /\
+    GVsSig.lift_op2 (mfbop TD b fp) gv1 gv2 (typ_floatpoint fp) = Some gv.
+Proof.
+  intros TD lc gl b fp v1 v2 gv HFBOP.
+  unfold FBOP in HFBOP.
+  remember (getOperandValue TD v1 lc gl) as ogv1.
+  destruct ogv1; try solve [inversion HFBOP].
+  remember (getOperandValue TD v2 lc gl) as ogv2.
+  destruct ogv2; inv HFBOP.
+  eauto.
+Qed.
+
+Lemma CAST_inversion : forall TD lc gl op t1 v1 t2 gv,
+  CAST TD lc gl op t1 v1 t2 = Some gv ->
+  exists gv1,
+    getOperandValue TD v1 lc gl = Some gv1 /\
+    GVsSig.lift_op1 (mcast TD op t1 t2) gv1 t2 = Some gv.
+Proof.
+  intros TD lc gl op t1 v1 t2 gv HCAST.
+  unfold CAST in HCAST.
+  remember (getOperandValue TD v1 lc gl) as ogv1.
+  destruct ogv1; inv HCAST.
+  eauto.
+Qed.
+
+Lemma TRUNC_inversion : forall TD lc gl op t1 v1 t2 gv,
+  TRUNC TD lc gl op t1 v1 t2 = Some gv ->
+  exists gv1,
+    getOperandValue TD v1 lc gl = Some gv1 /\
+    GVsSig.lift_op1 (mtrunc TD op t1 t2) gv1 t2 = Some gv.
+Proof.
+  intros TD lc gl op t1 v1 t2 gv HTRUNC.
+  unfold TRUNC in HTRUNC.
+  remember (getOperandValue TD v1 lc gl) as ogv1.
+  destruct ogv1; inv HTRUNC.
+  eauto.
+Qed.
+
+Lemma EXT_inversion : forall TD lc gl op t1 v1 t2 gv,
+  EXT TD lc gl op t1 v1 t2 = Some gv ->
+  exists gv1,
+    getOperandValue TD v1 lc gl = Some gv1 /\
+    GVsSig.lift_op1 (mext TD op t1 t2) gv1 t2 = Some gv.
+Proof.
+  intros TD lc gl op t1 v1 t2 gv HEXT.
+  unfold EXT in HEXT.
+  remember (getOperandValue TD v1 lc gl) as ogv1.
+  destruct ogv1; inv HEXT.
+  eauto.
+Qed.
+
+Lemma ICMP_inversion : forall TD lc gl cond t v1 v2 gv,
+  ICMP TD lc gl cond t v1 v2 = Some gv ->
+  exists gv1, exists gv2,
+    getOperandValue TD v1 lc gl = Some gv1 /\
+    getOperandValue TD v2 lc gl = Some gv2 /\
+    GVsSig.lift_op2 (micmp TD cond t) gv1 gv2 (typ_int 1%nat) = Some gv.
+Proof.
+  intros TD lc gl cond0 t v1 v2 gv HICMP.
+  unfold ICMP in HICMP.
+  remember (getOperandValue TD v1 lc gl) as ogv1.
+  destruct ogv1; try solve [inversion HICMP].
+  remember (getOperandValue TD v2 lc gl) as ogv2.
+  destruct ogv2; inv HICMP.
+  eauto.
+Qed.
+
+Lemma FCMP_inversion : forall TD lc gl cond fp v1 v2 gv,
+  FCMP TD lc gl cond fp v1 v2 = Some gv ->
+  exists gv1, exists gv2,
+    getOperandValue TD v1 lc gl = Some gv1 /\
+    getOperandValue TD v2 lc gl = Some gv2 /\
+    GVsSig.lift_op2 (mfcmp TD cond fp) gv1 gv2 (typ_int 1%nat) = Some gv.
+Proof.
+  intros TD lc gl cond0 fp v1 v2 gv HFCMP.
+  unfold FCMP in HFCMP.
+  remember (getOperandValue TD v1 lc gl) as ogv1.
+  destruct ogv1; try solve [inversion HFCMP].
+  remember (getOperandValue TD v2 lc gl) as ogv2.
+  destruct ogv2; inv HFCMP.
+  eauto.
+Qed.
+
+(*
+Lemma GEP_inversion : forall (TD:TargetData) (t:typ) (ma:GenericValue) 
+  (vidxs:list GenericValue) ib mptr0,
+  GEP TD t ma vidxs ib = Some mptr0 ->
+  exists idxs, exists ptr, exists ptr0, 
+    GVs2Nats TD vidxs = Some idxs /\ 
+    GV2ptr TD (getPointerSize TD) ma = Some ptr /\
+    mgep TD t ptr idxs = Some ptr0 /\
+    ptr2GV TD ptr0 = mptr0.
+Proof.
+  intros.
+  unfold GEP in H.
+  remember (GVs2Nats TD vidxs) as oidxs.
+  remember (GV2ptr TD (getPointerSize TD) ma) as R.
+  destruct R.
+    destruct oidxs.
+      remember (mgep TD t v l0) as og.
+      destruct og; inversion H; subst.
+        exists l0. exists v. exists v0. auto.
+        exists l0. exists v. exists v0. auto.
+
+Qed.
+*)
+
+Lemma const2GV_eqAL : forall c gl1 gl2 TD, 
+  eqAL _ gl1 gl2 -> 
+  const2GV TD gl1 c = const2GV TD gl2 c.
+Proof.
+  intros. unfold const2GV.
+  destruct const2GV_eqAL_aux.
+  erewrite H0; eauto.
+Qed.
+
+Lemma getOperandValue_eqAL : forall lc1 gl lc2 v TD,
+  eqAL _ lc1 lc2 ->
+  getOperandValue TD v lc1 gl = getOperandValue TD v lc2 gl.
+Proof.
+  intros lc1 gl lc2 v TD HeqAL.
+  unfold getOperandValue in *.
+  destruct v; auto.
+Qed.
+
+Lemma BOP_eqAL : forall lc1 gl lc2 bop0 sz0 v1 v2 TD,
+  eqAL _ lc1 lc2 ->
+  BOP TD lc1 gl bop0 sz0 v1 v2 = BOP TD lc2 gl bop0 sz0 v1 v2.
+Proof.
+  intros lc1 gl lc2 bop0 sz0 v1 v2 TD HeqEnv.
+  unfold BOP in *.
+  rewrite getOperandValue_eqAL with (lc2:=lc2)(v:=v1); auto.
+  rewrite getOperandValue_eqAL with (lc2:=lc2)(v:=v2); auto.
+Qed.
+
+Lemma FBOP_eqAL : forall lc1 gl lc2 fbop0 fp0 v1 v2 TD,
+  eqAL _ lc1 lc2 ->
+  FBOP TD lc1 gl fbop0 fp0 v1 v2 = FBOP TD lc2 gl fbop0 fp0 v1 v2.
+Proof.
+  intros lc1 gl lc2 fbop0 fp0 v1 v2 TD HeqEnv.
+  unfold FBOP in *.
+  rewrite getOperandValue_eqAL with (lc2:=lc2)(v:=v1); auto.
+  rewrite getOperandValue_eqAL with (lc2:=lc2)(v:=v2); auto.
+Qed.
+
+Lemma CAST_eqAL : forall lc1 gl lc2 op t1 v1 t2 TD,
+  eqAL _ lc1 lc2 ->
+  CAST TD lc1 gl op t1 v1 t2 = CAST TD lc2 gl op t1 v1 t2.
+Proof.
+  intros lc1 gl lc2 op t1 v1 t2 TD HeqAL.
+  unfold CAST in *.
+  rewrite getOperandValue_eqAL with (lc2:=lc2)(v:=v1); auto.
+Qed.
+
+Lemma TRUNC_eqAL : forall lc1 gl lc2 op t1 v1 t2 TD,
+  eqAL _ lc1 lc2 ->
+  TRUNC TD lc1 gl op t1 v1 t2 = TRUNC TD lc2 gl op t1 v1 t2.
+Proof.
+  intros lc1 gl lc2 op t1 v1 t2 TD HeqAL.
+  unfold TRUNC in *.
+  rewrite getOperandValue_eqAL with (lc2:=lc2)(v:=v1); auto.
+Qed.
+
+Lemma EXT_eqAL : forall lc1 gl lc2 op t1 v1 t2 TD,
+  eqAL _ lc1 lc2 ->
+  EXT TD lc1 gl op t1 v1 t2 = EXT TD lc2 gl op t1 v1 t2.
+Proof.
+  intros lc1 gl lc2 op t1 v1 t2 TD HeqAL.
+  unfold EXT in *.
+  rewrite getOperandValue_eqAL with (lc2:=lc2)(v:=v1); auto.
+Qed.
+
+Lemma ICMP_eqAL : forall lc1 gl lc2 cond t v1 v2 TD,
+  eqAL _ lc1 lc2 ->
+  ICMP TD lc1 gl cond t v1 v2 = ICMP TD lc2 gl cond t v1 v2.
+Proof.
+  intros lc1 gl lc2 cond0 t v1 v2 TD HeqAL.
+  unfold ICMP in *.
+  rewrite getOperandValue_eqAL with (lc2:=lc2)(v:=v1); auto.
+  rewrite getOperandValue_eqAL with (lc2:=lc2)(v:=v2); auto.
+Qed.
+
+Lemma FCMP_eqAL : forall lc1 gl lc2 cond fp v1 v2 TD,
+  eqAL _ lc1 lc2 ->
+  FCMP TD lc1 gl cond fp v1 v2 = FCMP TD lc2 gl cond fp v1 v2.
+Proof.
+  intros lc1 gl lc2 cond0 fp v1 v2 TD HeqAL.
+  unfold FCMP in *.
+  rewrite getOperandValue_eqAL with (lc2:=lc2)(v:=v1); auto.
+  rewrite getOperandValue_eqAL with (lc2:=lc2)(v:=v2); auto.
+Qed.
+
+Lemma values2GVs_eqAL : forall l0 lc1 gl lc2 TD,
+  eqAL _ lc1 lc2 ->
+  values2GVs TD l0 lc1 gl = values2GVs TD l0 lc2 gl.
+Proof.
+  induction l0; intros lc1 gl lc2 TD HeqAL; simpl; auto.
+    rewrite getOperandValue_eqAL with (lc2:=lc2)(v:=v); auto.
+    erewrite IHl0; eauto.
+Qed.
+(*
+Lemma lookupFdefViaGV_inversion : forall TD Ps gl lc fs fv f,
+  lookupFdefViaGV TD Ps gl lc fs fv = Some f ->
+  exists fptr, exists fn,
+    getOperandValue TD fv lc gl = Some fptr /\
+    lookupFdefViaGVFromFunTable fs fptr = Some fn /\
+    lookupFdefViaIDFromProducts Ps fn = Some f.
+Proof.
+  intros.
+  unfold lookupFdefViaGV in H.
+  destruct (getOperandValue TD fv lc gl); tinv H.
+  simpl in H. exists g.
+  destruct (lookupFdefViaGVFromFunTable fs g); tinv H.
+  simpl in H. exists i0. eauto.
+Qed.  
+*)
+
+End OpsemProps.
+
+(*****************************)
+(*
+*** Local Variables: ***
+*** coq-prog-name: "coqtop" ***
+*** coq-prog-args: ("-emacs-U" "-I" "~/SVN/sol/vol/src/ssa/monads" "-I" "~/SVN/sol/vol/src/ssa/ott" "-I" "~/SVN/sol/vol/src/ssa/compcert" "-I" "~/SVN/sol/theory/metatheory_8.3") ***
+*** End: ***
+ *)
